MiLkMaId_LiFtEr/Test_LiFtEr.thy
@@ -7,6 +7,8 @@ LiFtEr: Logical Feature Extractor.
 theory Test_LiFtEr
   imports
     "TIP_TO_Test_LiFtEr/Isaplanner/Isaplanner/TIP_prop_01"
+    "TIP_TO_Test_LiFtEr/TIP15/TIP15/TIP_list_count_nub"
+    "TIP_TO_Test_LiFtEr/TIP15/TIP15/TIP_propositional_AndCommutative"
 begin
 
 end
